examples/pseudo_bool/cp_encoding/cp_to_ilp_primScript.sml
@@ -5,7 +5,7 @@ Theory cp_to_ilp_prim
 Libs
   preamble
 Ancestors
-  pbc cp ilp cp_to_ilp
+  pbc pbc_encode cp ilp cp_to_ilp int_bitwise int_bitwiseExtra
 
 Definition cmk_eq_def[simp]:
   cmk_eq name X Y =
@@ -522,6 +522,356 @@ Proof
   intLib.ARITH_TAC
 QED
 
+(* Multiplication X * Y = Z by long multiplication on magnitudes;
+   binding spec: ENCODING_MULTIPLY.md *)
+
+(* bits needed for |v| with v ∈ [lb,ub]: |v| < 2 ** mult_width lb ub *)
+Definition mult_width_def:
+  mult_width lb ub =
+  LENGTH (bits_of_num (MAX (Num (ABS lb)) (Num (ABS ub))))
+End
+
+(* bit b of |X| (axis = 0) resp. |Y| (axis = 1) *)
+Definition mult_binbit_def[simp]:
+  mult_binbit name axis b = INR (name, Indices [axis; b] (SOME «bin»))
+End
+
+(* product flag: bit i of |X| AND bit j of |Y| *)
+Definition mult_prodbit_def[simp]:
+  mult_prodbit name i j = INR (name, Indices [i; j] (SOME «prod»))
+End
+
+(* BinRep(|X|) resp. BinRep(|Y|) as a positive bit sum *)
+Definition mult_bin_term_def:
+  mult_bin_term name axis w = pos_num (mult_binbit name axis) w
+End
+
+(* BinRep(|XY|) = Σ_{i<n,j<m} 2^(i+j) · prod_ij *)
+Definition mult_prod_term_def:
+  mult_prod_term pf n m =
+  FLAT (GENLIST (λi. GENLIST (λj. (&(2 ** (i + j)), Pos (pf i j))) m) n)
+End
+
+(* c·Zc + bs ≥ k, folding a constant Zc into the RHS *)
+Definition mult_varc_row_def:
+  mult_varc_row c Zc bs k =
+  case Zc of
+    INL v => ([(c,v)], bs, k)
+  | INR i => ([], bs, k - c * i)
+End
+
+(* the four [Zc≥0]-guarded rows pinning eval bs = |Zc| *)
+Definition mult_mag_rows_def:
+  mult_mag_rows bnd Zc bs =
+  let
+    g = Pos (INL (Ge Zc 0));
+    ng = Neg (INL (Ge Zc 0));
+    nbs = flip_coeffs bs
+  in
+  [
+    bits_imply bnd [g] (mult_varc_row 1 Zc nbs 0);
+    bits_imply bnd [g] (mult_varc_row (-1) Zc bs 0);
+    bits_imply bnd [ng] (mult_varc_row 1 Zc bs 0);
+    bits_imply bnd [ng] (mult_varc_row (-1) Zc nbs 0)
+  ]
+End
+
+(* All fresh rows (the reified atoms come separately, via the ec cache):
+   4 magnitude rows each for X, Y; n·m fully reified product flags;
+   4 rows pinning |Z| to BinRep(|XY|); 6 sign clauses. *)
+Definition cencode_mult_body_def:
+  cencode_mult_body bnd X Y Z name =
+  let
+    (lbx,ubx) = varc_bnd bnd X;
+    (lby,uby) = varc_bnd bnd Y;
+    n = mult_width lbx ubx;
+    m = mult_width lby uby;
+    xbs = mult_bin_term name 0 n;
+    ybs = mult_bin_term name 1 m;
+    pbs = mult_prod_term (mult_prodbit name) n m;
+    px0 = Pos (INL (Eq X 0));
+    py0 = Pos (INL (Eq Y 0));
+    px1 = Pos (INL (Ge X 1));
+    py1 = Pos (INL (Ge Y 1));
+    nx = Neg (INL (Ge X 0));
+    ny = Neg (INL (Ge Y 0));
+    zp = ([],[(1,Pos (INL (Ge Z 0)))],1);
+    zn = ([],[(1,Neg (INL (Ge Z 0)))],1)
+  in
+  Append
+    (List (mk_annotate
+      [mk_name name («Xge0_ge»); mk_name name («Xge0_le»);
+       mk_name name («Xlt0_ge»); mk_name name («Xlt0_le»)]
+      (mult_mag_rows bnd X xbs))) $
+  Append
+    (List (mk_annotate
+      [mk_name name («Yge0_ge»); mk_name name («Yge0_le»);
+       mk_name name («Ylt0_ge»); mk_name name («Ylt0_le»)]
+      (mult_mag_rows bnd Y ybs))) $
+  Append
+    (flat_app (GENLIST (λi.
+      flat_app (GENLIST (λj.
+        cbimply_var bnd (mult_prodbit name i j)
+          ([],[(1,Pos (mult_binbit name 0 i));
+               (1,Pos (mult_binbit name 1 j))],2)) m)) n)) $
+  Append
+    (List (mk_annotate
+      [mk_name name («mag_Zge0_ge»); mk_name name («mag_Zge0_le»);
+       mk_name name («mag_Zlt0_ge»); mk_name name («mag_Zlt0_le»)]
+      (mult_mag_rows bnd Z pbs))) $
+    (List (mk_annotate
+      [mk_name name («sgn_x0»); mk_name name («sgn_y0»);
+       mk_name name («sgn_pp»); mk_name name («sgn_nn»);
+       mk_name name («sgn_np»); mk_name name («sgn_pn»)]
+      [
+        bits_imply bnd [px0] zp;
+        bits_imply bnd [py0] zp;
+        bits_imply bnd [px1; py1] zp;
+        bits_imply bnd [nx; ny] zp;
+        bits_imply bnd [nx; py1] zn;
+        bits_imply bnd [px1; ny] zn
+      ]))
+End
+
+Definition cencode_mult_def:
+  cencode_mult bnd X Y Z name ec =
+  let
+    (e1,ec1) = cencode_full_eq bnd X 0 ec;
+    (e2,ec2) = cencode_full_eq bnd Y 0 ec1;
+    (e3,ec3) = cencode_ge bnd Z 0 ec2
+  in
+    (Append e1 $ Append e2 $ Append e3 $
+      cencode_mult_body bnd X Y Z name, ec3)
+End
+
+Definition encode_mult_def:
+  encode_mult bnd X Y Z name =
+  encode_full_eq bnd X 0 ++
+  encode_full_eq bnd Y 0 ++
+  encode_ge bnd Z 0 ++
+  abstr (cencode_mult_body bnd X Y Z name)
+End
+
+Theorem mult_varc_row_sem[local,simp]:
+  iconstraint_sem (mult_varc_row c Zc bs k) (wi,wb) ⇔
+  c * varc wi Zc + eval_lin_term wb bs ≥ k
+Proof
+  rw[mult_varc_row_def]>>
+  every_case_tac>>
+  simp[iconstraint_sem_def,eval_ilin_term_def,iSUM_def,varc_def]>>
+  intLib.ARITH_TAC
+QED
+
+(* given an exact [Zc ≥ 0] atom, the four rows pin eval bs to |Zc| *)
+Theorem mult_mag_rows_sem[local]:
+  valid_assignment bnd wi ∧
+  (wb (INL (Ge Zc 0)) ⇔ varc wi Zc ≥ 0) ⇒
+  (EVERY (λx. iconstraint_sem x (wi,wb)) (mult_mag_rows bnd Zc bs) ⇔
+   eval_lin_term wb bs = ABS (varc wi Zc))
+Proof
+  rw[mult_mag_rows_def]>>
+  Cases_on ‘wb (INL (Ge Zc 0))’>>
+  gvs[]>>
+  intLib.ARITH_TAC
+QED
+
+Theorem mult_width_bound[local]:
+  valid_assignment bnd wi ∧ varc_bnd bnd X = (lb,ub) ⇒
+  Num (ABS (varc wi X)) < 2 ** mult_width lb ub
+Proof
+  simp[mult_width_def]>>
+  namedCases_on ‘X’ ["v","c"]>>
+  gvs[varc_bnd_def,varc_def]
+  >- (
+    rw[valid_assignment_def]>>
+    first_x_assum (qspec_then ‘v’ mp_tac)>>
+    simp[]>>strip_tac>>
+    ‘Num (ABS (wi v)) ≤ MAX (Num (ABS lb)) (Num (ABS ub))’ by
+      (rw[MAX_DEF]>>intLib.ARITH_TAC)>>
+    metis_tac[LESS_LENGTH_bits_of_num,LESS_EQ_LESS_TRANS])>>
+  rw[]>>gvs[MAX_DEF]>>
+  metis_tac[LESS_LENGTH_bits_of_num]
+QED
+
+(* reified magnitude bits evaluate back to |v| *)
+Theorem mult_bin_eval[local]:
+  Num (ABS v) < 2 ** w ∧
+  (∀b. b < w ⇒ (wb (flag b) ⇔ BIT b (Num (ABS v)))) ⇒
+  eval_lin_term wb (pos_num flag w) = ABS v
+Proof
+  rw[]>>
+  drule_all pos_num_reify_eq>>
+  rw[]>>
+  intLib.ARITH_TAC
+QED
+
+Theorem mult_two_pos_sem[local,simp]:
+  iconstraint_sem ([],[(1,Pos a);(1,Pos b)],2) (wi,wb) ⇔ wb a ∧ wb b
+Proof
+  simp[eval_lin_term_def,iSUM_def]>>
+  Cases_on ‘wb a’>>Cases_on ‘wb b’>>simp[]
+QED
+
+(* one row of the long multiplication *)
+Theorem eval_mult_prod_row[local]:
+  ∀m.
+  (∀j. j < m ⇒ (wb (pf j) ⇔ g ∧ wb (by j))) ⇒
+  eval_lin_term wb (GENLIST (λj. (&(2 ** (i + j)), Pos (pf j))) m) =
+  &(2 ** i) * b2i g * eval_lin_term wb (pos_num by m)
+Proof
+  Induct>>
+  rw[pos_num_def,GENLIST,SNOC_APPEND]>>
+  Cases_on ‘g’>>Cases_on ‘wb (by m)’>>
+  gvs[EXP_ADD,integerTheory.INT_LDISTRIB]
+QED
+
+(* AND-reified product flags: the shifted sum multiplies out, for ANY bits *)
+Theorem eval_mult_prod_term[local]:
+  ∀n.
+  (∀i j. i < n ∧ j < m ⇒ (wb (pf i j) ⇔ wb (bx i) ∧ wb (by j))) ⇒
+  eval_lin_term wb (mult_prod_term pf n m) =
+  eval_lin_term wb (pos_num bx n) * eval_lin_term wb (pos_num by m)
+Proof
+  Induct>>
+  rw[mult_prod_term_def,pos_num_def,GENLIST,SNOC_APPEND]>>
+  gvs[GSYM pos_num_def,GSYM mult_prod_term_def]>>
+  ‘eval_lin_term wb (GENLIST (λj. (&(2 ** (j + n)),Pos (pf n j))) m) =
+   &(2 ** n) * b2i (wb (bx n)) * eval_lin_term wb (pos_num by m)’ by
+    (once_rewrite_tac[arithmeticTheory.ADD_COMM]>>
+     irule eval_mult_prod_row>>rw[])>>
+  simp[integerTheory.INT_RDISTRIB]
+QED
+
+Theorem mult_prod_block_sem[local]:
+  valid_assignment bnd wi ⇒
+  (EVERY (λx. iconstraint_sem x (wi,wb))
+    (FLAT (MAP (λls. abstr ls)
+      (GENLIST (λi.
+        flat_app (GENLIST (λj.
+          cbimply_var bnd (INR (name,Indices [i; j] (SOME «prod»)))
+            ([],[(1,Pos (INR (name,Indices [0; i] (SOME «bin»))));
+                 (1,Pos (INR (name,Indices [1; j] (SOME «bin»))))],2)) m)) n))) ⇔
+   ∀i j. i < n ∧ j < m ⇒
+     (wb (INR (name,Indices [i; j] (SOME «prod»))) ⇔
+      wb (INR (name,Indices [0; i] (SOME «bin»))) ∧
+      wb (INR (name,Indices [1; j] (SOME «bin»)))))
+Proof
+  rw[append_flat_app,EVERY_FLAT,EVERY_MAP,EVERY_GENLIST,cbimply_var_def]>>
+  metis_tac[]
+QED
+
+Theorem mult_sign_facts[local]:
+  ((x:int) = 0 ⇒ x * y ≥ 0) ∧ (y = 0 ⇒ x * y ≥ 0) ∧
+  (x ≥ 1 ∧ y ≥ 1 ⇒ x * y ≥ 0) ∧
+  (¬(x ≥ 0) ∧ ¬(y ≥ 0) ⇒ x * y ≥ 0) ∧
+  (¬(x ≥ 0) ∧ y ≥ 1 ⇒ ¬(x * y ≥ 0)) ∧
+  (x ≥ 1 ∧ ¬(y ≥ 0) ⇒ ¬(x * y ≥ 0))
+Proof
+  rw[integerTheory.INT_GE,integerTheory.INT_NOT_LE]>>
+  simp[integerTheory.INT_MUL_SIGN_CASES,integerTheory.INT_LE_LT]>>
+  intLib.ARITH_TAC
+QED
+
+Theorem mult_abs_sign_eq[local]:
+  ABS z = ABS p ∧ (0 < p ∧ z ≥ 0 ∨ p < 0 ∧ ¬(z ≥ 0) ∨ p = 0) ⇒ z = p
+Proof
+  intLib.ARITH_TAC
+QED
+
+(* |z| = |x·y| plus the four sign clauses force z = x·y *)
+Theorem mult_sign_bridge[local]:
+  ABS z = ABS (x * y) ∧
+  (x ≥ 1 ∧ y ≥ 1 ⇒ z ≥ 0) ∧
+  (¬(x ≥ 0) ∧ ¬(y ≥ 0) ⇒ z ≥ 0) ∧
+  (¬(x ≥ 0) ∧ y ≥ 1 ⇒ ¬(z ≥ 0)) ∧
+  (x ≥ 1 ∧ ¬(y ≥ 0) ⇒ ¬(z ≥ 0)) ⇒
+  z = x * y
+Proof
+  strip_tac>>
+  irule mult_abs_sign_eq>>
+  simp[]>>
+  simp[integerTheory.INT_MUL_SIGN_CASES]>>
+  Cases_on ‘0 < x’>>Cases_on ‘0 < y’>>gvs[]>>
+  qpat_x_assum ‘ABS _ = _’ kall_tac>>
+  intLib.ARITH_TAC
+QED
+
+Theorem encode_mult_sem_1:
+  valid_assignment bnd wi ∧
+  ALOOKUP cs name = SOME (Prim (Nonlinop Mult X Y Z)) ∧
+  varc wi X * varc wi Y = varc wi Z ⇒
+  EVERY (λx. iconstraint_sem x (wi,reify_avar cs wi))
+    (encode_mult bnd X Y Z name)
+Proof
+  rw[encode_mult_def]>>
+  simp[reify_avar_def,reify_reif_def]>>
+  rw[cencode_mult_body_def]>>rpt(pairarg_tac>>gvs[])>>
+  simp[mult_mag_rows_sem,reify_avar_def,reify_reif_def]>>
+  ‘∀b. b2i b ≥ 1 ⇔ b’ by (Cases>>simp[])>>
+  simp[]>>
+  simp[mult_sign_facts]>>
+  qpat_x_assum ‘_ * _ = varc _ _’ (assume_tac o GSYM)>>
+  gvs[mult_sign_facts]>>
+  ‘∀ax b. reify_avar cs wi (INR (name,Indices [ax; b] (SOME «bin»))) ⇔
+     BIT b (Num (ABS (varc wi (if ax = 0 then X else Y))))’ by
+    gvs[reify_avar_def,reify_flag_def]>>
+  ‘∀i j. reify_avar cs wi (INR (name,Indices [i; j] (SOME «prod»))) ⇔
+     BIT i (Num (ABS (varc wi X))) ∧ BIT j (Num (ABS (varc wi Y)))’ by
+    gvs[reify_avar_def,reify_flag_def]>>
+  ‘eval_lin_term (reify_avar cs wi)
+     (pos_num (mult_binbit name 0) (mult_width lbx ubx)) = ABS (varc wi X)’ by
+    (irule mult_bin_eval>>fs[]>>metis_tac[mult_width_bound])>>
+  ‘eval_lin_term (reify_avar cs wi)
+     (pos_num (mult_binbit name 1) (mult_width lby uby)) = ABS (varc wi Y)’ by
+    (irule mult_bin_eval>>fs[]>>metis_tac[mult_width_bound])>>
+  ‘eval_lin_term (reify_avar cs wi)
+     (mult_prod_term (mult_prodbit name) (mult_width lbx ubx)
+        (mult_width lby uby)) =
+   eval_lin_term (reify_avar cs wi)
+     (pos_num (mult_binbit name 0) (mult_width lbx ubx)) *
+   eval_lin_term (reify_avar cs wi)
+     (pos_num (mult_binbit name 1) (mult_width lby uby))’ by
+    (irule eval_mult_prod_term>>fs[])>>
+  simp[mult_bin_term_def,GSYM integerTheory.INT_ABS_MUL]>>
+  rw[EVERY_FLAT,EVERY_MAP,EVERY_GENLIST,cbimply_var_def]>>
+  rw[append_flat_app,EVERY_FLAT,EVERY_MAP,EVERY_GENLIST]>>fs[]
+QED
+
+Theorem encode_mult_sem_2:
+  valid_assignment bnd wi ∧
+  EVERY (λx. iconstraint_sem x (wi,wb))
+    (encode_mult bnd X Y Z name) ⇒
+  varc wi X * varc wi Y = varc wi Z
+Proof
+  rw[encode_mult_def]>>
+  fs[cencode_mult_body_def]>>rpt(pairarg_tac>>gvs[])>>
+  gs[mult_mag_rows_sem,mult_prod_block_sem]>>
+  ‘∀b. b2i b ≥ 1 ⇔ b’ by (Cases>>simp[])>>
+  fs[mult_bin_term_def]>>
+  ‘eval_lin_term wb (mult_prod_term (mult_prodbit name) (mult_width lbx ubx)
+     (mult_width lby uby)) =
+   eval_lin_term wb (pos_num (mult_binbit name 0) (mult_width lbx ubx)) *
+   eval_lin_term wb (pos_num (mult_binbit name 1) (mult_width lby uby))’ by
+    (irule eval_mult_prod_term>>fs[])>>
+  gvs[GSYM integerTheory.INT_ABS_MUL]>>
+  once_rewrite_tac[EQ_SYM_EQ]>>
+  irule mult_sign_bridge>>
+  simp[]>>
+  metis_tac[integerTheory.INT_ABS_MUL]
+QED
+
+Theorem cencode_mult_sem:
+  valid_assignment bnd wi ∧
+  cencode_mult bnd X Y Z name ec = (es, ec') ⇒
+  enc_rel wi es (encode_mult bnd X Y Z name) ec ec'
+Proof
+  rw[cencode_mult_def,encode_mult_def]>>
+  gvs[UNCURRY_EQ]>>
+  pure_rewrite_tac[GSYM APPEND_ASSOC]>>
+  metis_tac[enc_rel_Append,enc_rel_encode_full_eq,
+    enc_rel_encode_ge,enc_rel_abstr]
+QED
+
 Definition encode_prim_constr_def:
   encode_prim_constr bnd c name =
   case c of
@@ -541,6 +891,9 @@ Definition encode_prim_constr_def:
       | Minus => encode_minus X Y Z
       | Min => encode_min bnd X Y Z name
       | Max => encode_max bnd X Y Z name)
+  | Nonlinop nlop X Y Z =>
+      (case nlop of
+        Mult => encode_mult bnd X Y Z name)
 End
 
 Theorem encode_prim_constr_sem_1:
@@ -557,6 +910,8 @@ Proof
   >- (Cases_on`p`>>gvs[]>>
       metis_tac[encode_plus_sem_1,encode_minus_sem_1,
                 encode_min_sem_1,encode_max_sem_1])
+  >- (Cases_on`p`>>gvs[nlop_sem_def,nlop_val_def]>>
+      metis_tac[encode_mult_sem_1])
   >- (irule encode_equal_sem_1>>
       gvs[cmpop_sem_def,cmpop_val_def])
   >- (irule encode_not_equal_sem_1>>
@@ -577,6 +932,8 @@ Proof
   >- (Cases_on`p`>>gvs[]>>
       metis_tac[encode_plus_sem_2,encode_minus_sem_2,
                 encode_min_sem_2,encode_max_sem_2])
+  >- (Cases_on`p`>>gvs[nlop_sem_def,nlop_val_def]>>
+      metis_tac[encode_mult_sem_2])
   >- (gvs[cmpop_sem_def,cmpop_val_def]>>
       metis_tac[encode_equal_sem_2])
   >- (gvs[cmpop_sem_def,cmpop_val_def]>>
@@ -749,6 +1106,9 @@ Definition cencode_prim_constr_def:
     | Max => (cencode_max bnd X Y Z name, ec)
     | Plus => (cencode_plus bnd X Y Z name, ec)
     | Minus => (cencode_minus bnd X Y Z name, ec))
+  | Nonlinop nlop X Y Z =>
+    (case nlop of
+      Mult => cencode_mult bnd X Y Z name ec)
 End
 
 Theorem cencode_prim_constr_sem:
@@ -770,6 +1130,7 @@ Proof
   >- simp[cencode_minus_def,encode_minus_def,enc_rel_List_mk_annotate]
   >- simp[encode_min_def]
   >- simp[encode_max_def]
+  >- metis_tac[cencode_mult_sem]
   >- metis_tac[cencode_equal_sem]
   >- metis_tac[cencode_not_equal_sem]
   >- metis_tac[cencode_order_cmpops_sem]
